\documentclass[a4paper,11pt,onepage]{article}

\usepackage[utf8]{inputenc}
\usepackage{graphicx}
\usepackage{amsmath}
\newcommand{\cov}{\mathrm{cov}}

\newcommand{\ddp}[2]{\frac{\partial #1}{\partial #2}}

\begin{document}
 

%---------------------------------------------------------------------------------------------
%
%------------------------------- TOTAL LEAST SQUARES --------------------------------------------------
%
%---------------------------------------------------------------------------------------------
\section{Total least squares - long not in documentation} \label{tls}
The total (orthogonal) least squares regression is an optimization method to fit the data $(x_i, y_i)$ with a function $f(x_i;\beta_a)$, $\beta_a$ being the (unknown) parameters.
It is based on the minimization of the sum of (orthogonal) distances of datapoints from the curve 
\begin{equation*}
 S = \sum_{i=1}^n w_i \left[(y_i - f(x_i^*; \beta_a))^2 + \delta_i (x_i - x_i^*)^2 \right],
\end{equation*} 
where $\delta = \sigma_{y}/\sigma_{x}$ is the ratio of the error variances in $x$ and $y$, $w_i$ are weights of the points and the values $x_i^*$ are parameters corresponding to the ``true'' x-values of the points on the curve. \\

\subsection{total least squares: straight line}
In general this leads to a set of nonlinear equations which must be solved numerically. For a straight line with equal weights $w_i=1$  and uniform error estimates $\delta_i = \delta$

\begin{equation}
 y = f(x) = ax +b,
\end{equation}
the problem can be solved analytically. The derivatives of $S$ with respect to the parameters $a$, $b$ and $x_i^*$ are
\begin{eqnarray*}
 \ddp{S}{a} &=& \sum_{i=1}^n 2(y_i - ax_i^* -b) (-x_i^*) \\
 \ddp{S}{b} &=& \sum_{i=1}^n 2 (y_i - ax_i^* -b) (-1) \\
 \ddp{S}{x_i^*} &=& 2 (y_i -ax_i^* -b) (-a) + 2 \delta(x_i - x_i^*) (-1),
\end{eqnarray*}
they must be all set to zero (to find the minimum). Thus we start with the system of equations
\begin{eqnarray}
 \sum_{i=1}^n y_i x_i^* - a \sum_{i=1}^n \left(x_i^*\right)^2 -b\sum_{i=1}^n x_i^* &=&  0\label{eq:tls_dS_1}\\
 \sum_{i=1}^n y_i - a \sum_{i=1}^n x_i^* -bn &=& 0 \label{eq:tls_dS_2} \\
 a(y_i -ax_i^* -b)  + \delta(x_i - x_i^*) &=& 0. \label{eq:tls_dS_3}
\end{eqnarray}
Express $x_i^*$ from \eqref{eq:tls_dS_3} as
\begin{equation}
 x_i^* = \frac1{\delta +a^2} \left( \delta x_i + a y_i - ab\right) = x_i + \frac{a}{\delta+a^2} \left( y_i -b - a x_i \right)
\end{equation}
and calculate the sums $\sum_i x_i^*$, $\sum_i \left(x_i^*\right)^2$ and $\sum_{i=1}^n x_i^* y_i$
\begin{eqnarray}
 \sum_{i=1}^n x_i^* &=& \sum_{i=1}^n  x_i + \frac{a}{\delta+a^2} \left( y_i - ax_i - b\right) \nonumber \\
 &=& n \bar x + \frac{na}{\delta+a^2} \left(  \bar y - a  \bar x - b\right) \label{eq:tls_sum_xstar}
\end{eqnarray}
\begin{eqnarray}
 \sum_{i=1}^n \left( x_i^*\right)^2 &=& \sum_{i=1}^n x_i^2 + \frac{2a}{\delta+a^2} \left( x_i y_i -a x_i^2 -b x_i \right) + \frac{a^2}{(\delta+a^2)^2} \left( y_i - a x_i -b \right)^2 \nonumber\\
 &=& \sum_{i=1}^n x_i^2 + \frac{2a}{\delta+a^2} \sum_{i=1}^n x_i y_i - \frac{2a^2 }{\delta+a^2} \sum_{i=1}^n x_i^2 - \frac{2ab}{\delta+a^2} n\bar x + \nonumber\\
 &&+ \frac{a^2}{(\delta+a^2)^2} \sum_{i=1}^n y_i^2 + \frac{a^4}{(\delta+a^2)^2} \sum_{i=1}^n x_i^2 + \frac{a^2}{(\delta+a^2)^2} b^2 n + \nonumber\\
 &&- \frac{2a^3}{(\delta+a^2)^2} \sum_{i=1}^n y_i x_i - \frac{2a^2b}{(\delta+a^2)^2} n \bar y + \frac{2a^3b}{(\delta+a^2)^2} n \bar x \nonumber \\
 &=& \frac{a^2}{(\delta+a^2)^2} \sum_{i=1}^n y_i^2 +
 \frac{2a \delta}{(\delta+a^2)^2} \sum_{i=1}^n x_i y_i   + 
 \sum_{i=1}^n x_i^2 \left[ 1 - \frac{2a^2 }{\delta+a^2}  + \frac{a^4}{(\delta+a^2)^2} \right] + \nonumber\\
&& - \frac{2a^2b}{(\delta+a^2)^2} n \bar y  - \frac{2ab\delta}{(\delta+a^2)^2} n \bar x + \frac{a^2}{(\delta+a^2)^2} b^2 n = \nonumber\\
&=& \frac1{(\delta+a^2)^2} \left[ a^2 \sum_{i=1}^n y_i^2 + 2a \delta \sum_{i=1}^n x_i y_i + \delta^2\sum_{i=1}^n x_i^2
-2 a^2b n \bar y  - 2 ab \delta n \bar x + a^2 b^2 n \right] \nonumber \\
&=& \frac{n}{(\delta+a^2)^2} \left[ a^2 \overline{ y^2}  + 2a \delta \overline{xy} + \delta^2 \overline{x^2} 
-2 a^2b  \bar y  - 2 ab \delta \bar x + a^2 b^2  \right] \label{eq:tls_sum_xstar^2}
\end{eqnarray}
\begin{eqnarray*}
 \sum_{i=1}^n x_i^* y_i &=& 
 \sum_{i=1}^n  y_i  x_i + \frac{a}{\delta+a^2}\sum_{i=1}^n \left(y_i^2\right)^2 - \frac{ab}{\delta+a^2}\sum_{i=1}^n y_i - \frac{a^2}{\delta+a^2} \sum_{i=1}^n x_i y_i \\
 &=& n \frac1{\delta+a^2} \left [\delta \overline{xy} + a \overline{y^2} - ab\bar y \right]
\end{eqnarray*}

Divide equation \eqref{eq:tls_dS_2} by $n$ and insert to find
\begin{eqnarray}
 0 &=& \bar y - a \left[  \bar x + \frac{a}{\delta+a^2} \left(  \bar y - a  \bar x - b\right) \right] -b \nonumber \\
  0 &=& \frac{\delta}{\delta+a^2} \bar y - \frac{a \delta}{\delta+a^2} \bar x - b \frac{\delta}{\delta+a^2} \nonumber\\
  0 &=& \bar y - a \bar x -b \label{eq:tls_xbarybar}
\end{eqnarray}

Divide equation \eqref{eq:tls_dS_1} by $n$ and insert the sums
\begin{eqnarray*}
 0 &=&
  \frac1{\delta+a^2} \left [ \delta \overline{xy} + a \overline{y^2} - ab\bar y \right] \\
&&  - \frac{a}{(\delta+a^2)^2} \left[ a^2 \overline{ y^2}  + 2a\delta \overline{xy} + \delta^2\overline{x^2}  
-2 a^2b  \bar y  - 2 ab \delta \bar x + a^2 b^2  \right] \\
&&- b \left[  \bar x + \frac{a}{\delta+a^2} \left(  \bar y - a  \bar x - b\right) \right] \\	
&=& \frac1{(\delta+a^2)^2} \left[ \delta a \overline{y^2} + (\delta^2 - \delta a^2 )\overline{xy} -a \delta^2 \overline{x^2} -(\delta-a^2)ab \bar y - (\delta^2+a^4 )  b \bar x -a^3 b^2
\right]
\end{eqnarray*}
where we used also \eqref{eq:tls_xbarybar}. Expressing $b$ from \eqref{eq:tls_xbarybar} as $ b = \bar y - a \bar x$ and multiplying the whole equation with $(\delta+a^2)^2$ we get
\begin{eqnarray*}
 0 &=& \delta a \overline{y^2} + \delta(\delta -a^2 )\overline{xy} -a \delta^2 \overline{x^2} -(\delta-a^2)a \bar y ( \bar y - a \bar x) - (\delta^2+ a^4)  \bar x ( \bar y - a \bar x) -a^3 (\bar y - a \bar x)^2\\
 %
 &=& \delta a \overline{y^2} + \delta (\delta -a^2 )\overline{xy} -a \delta^2 \overline{x^2} -(\delta-a^2)a \left(\bar y\right)^2  +(\delta-a^2) a^2 \bar x\bar y - (\delta+ a^4)  \bar x \bar y \\
 &&+ (\delta^2+ a^4)a \left(\bar x\right)^2 -a^3 (\bar y)^2 +2 a^4 \bar x \bar y - a^5 \left( \bar x \right)^2 \\
 %
 &=& \delta a \overline{y^2} - \delta a \left(\bar y\right)^2+ \delta (\delta -a^2 )\overline{xy} - \delta \left[ \delta - a^2\right] \bar x\bar y -a \delta^2 \overline{x^2} +a \delta^2\left( \bar x \right)^2 \\
 &=& \delta a s_{yy} + \delta (\delta-a^2) s_{xy} -a \delta^2s_{xx}
\end{eqnarray*}
where
\begin{eqnarray*}
 s_{xx} &=& \overline{x^2} - \left(\bar x \right)^2 = \frac1n \sum_{i=1}^n \left( x_i - \bar x \right)^2 \\%= \frac1n \sum_{i=1}^n \left( x_i^2 -2x_i \bar x + (\bar x)^2 \right)\\
 s_{xy} &=& \overline{xy} - \bar x \bar y  = \frac1n \sum_{i=1}^n \left( x_i - \bar x \right) \left( y_i - \bar y \right) \\
 s_{yy} &=& \overline{y^2} - \left(\bar y \right)^2 = \frac1n \sum_{i=1}^n \left( y_i - \bar y \right)^2.
 \end{eqnarray*}
For $\delta \neq 0$ this is a quadratic equation in $a$ with the solution
\begin{equation}
 a = \frac1{2 s_{xy}} \left[ s_{yy}- \delta s_{xx} \pm \sqrt{ ( s_{yy} - \delta s_{xx})^2 + 4 \delta s_{xy}^2} \right]
\end{equation}
We choose the upper sign in order to get the correct limit for $\delta \rightarrow 0$ which corresponds to ordinary least squares.
The final solution is thus
\begin{eqnarray}
 a &=& \frac1{2 s_{xy}} \left[ s_{yy}- \delta s_{xx} + \sqrt{ ( s_{yy} - \delta s_{xx})^2 + 4 \delta s_{xy}^2} \right] \\
 b &=& \bar y -a \bar x \\
 x_i^* &=& \frac1{\delta+a^2} \left( x_i + a y_i - ab\right) = x_i + \frac{a}{\delta+a^2} \left( y_i -b - a x_i \right)
 \end{eqnarray}
 
\subsection{total least squares, uncertainties a la GUM}
Uncertainties can be calculated by two ways: either using the law of propagation or as the inverse of the Hessian matrix (partial derivatives of the sum of squares with respect to the parameters).
By calculating explicitly all derivatives
\begin{eqnarray}
 u(a)^2 &=& \underbrace{\sum_{i=1}^n \left(\ddp{a}{x_i}\right)^2 u(x_i)^2}_{u(a;x)^2} + \underbrace{\sum_{i=1}^n \left(\ddp{a}{y_i}\right)^2 u(y_i)^2}_{u(a;y)^2} \\
 u(b)^2 &=& \underbrace{\sum_{i=1}^n \left(\ddp{b}{x_i}\right)^2 u(x_i)^2}_{u(b;x)^2} + \underbrace{\sum_{i=1}^n \left(\ddp{b}{y_i}\right)^2 u(y_i)^2}_{u(b;y)^2} \\
 \cov(a,b) &=& \underbrace{ \sum_{i=1}^n \ddp{a}{x_i} \ddp{b}{x_i} u(x_i)^2 }_{\cov(a,b;x)} + \underbrace{\sum_{i=1}^n \ddp{a}{y_i} \ddp{b}{y_i} u(y_i)^2}_{\cov(a,b;y)}
 \end{eqnarray}
We start with the uncertainty of the slope. Use the chain rule to write the derivatives in terms of the $s_{xx}$ etc. 
\begin{eqnarray*}
 \ddp{a}{x_i} &=& \ddp{a}{s_{xx}} \ddp{s_{xx}}{x_i} + \ddp{a}{s_{xy}} \ddp{s_{xy}}{x_i} \\
 \ddp{a}{y_i} &=& \ddp{a}{s_{yy}} \ddp{s_{yy}}{y_i} + \ddp{a}{s_{xy}} \ddp{s_{xy}}{y_i} 
 \end{eqnarray*}
First note that 
\begin{eqnarray*}
 \ddp{\bar x}{x_i} &=& \ddp{}{x_i} \frac1n \sum_{k=1}^n x_k = \frac1n \sum_{k=1}^n \delta_{ik} = \frac1n,
\end{eqnarray*}
and analoguously for $y$.
The derivatives of the $s_{xx}$ and $s_{xy}$ with respect to $x$ are simply
\begin{eqnarray*}
 \ddp{s_{xx}}{x_i} &=& \ddp{}{x_i} \sum_{j=1}^n \frac1n \left(x_j - \bar x \right)^2 \\
 &=& \frac2n \sum_{j=1} \left( x_j - \bar x \right) \left( \delta_{ij} - \frac1n \right) \\
 &=& \frac2n \sum_{j=1} \left( x_j - \bar x \right)\delta_{ij}  - \frac{2}{n^2} \underbrace{\sum_{j=1} \left( x_j -\bar x \right) }_{=0} \\
 &=& \frac2n  \left( x_i - \bar x \right)
\end{eqnarray*}
and 
\begin{eqnarray*}
 \ddp{s_{xy}}{x_i} &=& \ddp{}{x_i} \sum_{j=1}^n \frac1n \left(x_j - \bar x \right) \left( y_j - \bar y \right) \\
&=& \frac1n \sum_{j=1}^n \left( \delta_{ij} - \frac1n \right) \left(y_j - \bar y \right) \\
&=& \frac1n \sum_{j=1}^n \delta_{ij} \left(y_j - \bar y \right) - \frac1{n^2} \sum_{j=1}^n \left(y_j - \bar y \right)	\\
&=& \frac1n \left(y_i - \bar y \right)
\end{eqnarray*}
The other derivatives are analoguous.\\
The derivatives of the slope with respect to the $s_{xx}$ etc. are 
\begin{eqnarray*}
 \ddp{a}{s_{xx}} &= & \frac1{2s_{xy}} \left[ - \delta +  \frac12 \frac1{\sqrt{( s_{yy} - \delta s_{xx})^2 + 4 \delta s_{xy}^2}} 2 (s_{yy}-\delta s_{xx}) (-\delta)\right] \\
     &=& -\frac\delta{2s_{xy}} \left[ 1 + \frac{s_{yy}- \delta s_{xx}}{\sqrt{( s_{yy} -\delta s_{xx})^2 + 4 \delta s_{xy}^2}} \right] \\
     %
 \ddp{a}{s_{yy}} &=& \frac1{2s_{xy}} \left[ 1 + \frac{s_{yy}- \delta s_{xx}}{\sqrt{( s_{yy} - \delta s_{xx})^2 + 4 \delta s_{xy}^2}} \right] \\
 %
 \ddp{a}{s_{xy}} &=& -\frac1{2s_{xy}^2} \left[ s_{yy}- \delta s_{xx} + \sqrt{ ( s_{yy} - \delta s_{xx})^2 + 4 \delta s_{xy}^2} \right] + \\
 && + \frac1{2s_{xy}} \frac12 \frac1{\sqrt{ ( s_{yy} - \delta s_{xx})^2 + 4 \delta s_{xy}^2}} 8 \delta s_{xy} \\
 %
 &=&-\frac1{2s_{xy}^2} \left[ s_{yy}- \delta s_{xx} \right] + \\
 &&-\frac1{2s_{xy}^2} \frac1{\sqrt{ ( s_{yy} - \delta s_{xx})^2 + 4 \delta s_{xy}^2}} \left[ ( s_{yy} - \delta s_{xx})^2 + 4 \delta s_{xy}^2 - 4 \delta s_{xy}^2 \right] \\
 %
 &=& -\frac1{2s_{xy}^2} \left[ s_{yy}- \delta s_{xx} \right] -\frac1{2s_{xy}^2} \frac{ ( s_{yy} - \delta s_{xx})^2}{\sqrt{ ( s_{yy} - \delta s_{xx})^2 + 4 \delta s_{xy}^2}} 
\end{eqnarray*}
The derivatives of intercept  are
\begin{eqnarray*}
 \ddp{b}{x_i} &=& - \ddp{a}{x_i} \bar x - a \frac1n \\
 \ddp{b}{y_i} &=& \frac1n - \ddp{a}{y_i} \bar x
\end{eqnarray*}

If the variances are the same for all $x_i$ and $y_i$ we can simplify the previous expressoins
\begin{eqnarray*}
 u(a;x)^2 &=& \sum_{i=1}^n \left(\ddp{a}{x_i}\right)^2 u(x_i)^2 \\
 &=& \sum_{i=1}^n \left( \ddp{a}{s_{xx}} \ddp{s_{xx}}{x_i} + \ddp{a}{s_{xy}} \ddp{s_{xy}}{x_i}\right)^2 u(x)^2 \\
 &=& u(x)^2 \sum_{i=1}^n \left[ \left( \ddp{a}{s_{xx}}  \frac2{n} (x_i - \bar x) \right)^2  + \right. 
      2\ddp{a}{s_{xx}} \ddp{a}{s_{xy}} \frac2n (x_i - \bar x ) \frac1n (y_i - \bar y) \\
        && \left.+ \left( \ddp{a}{s_{xy}} \frac1n (y_i - \bar y) \right)^2 
       \right] \\
 &=& u(x) ^2 \left[ \left( \ddp{a}{s_{xx}} \right)^2 \frac4{n} s_{xx} +  \ddp{a}{s_{xx}} \ddp{a}{s_{xy}} \frac4n s_{xy} 
 + \left( \ddp{a}{s_{xy}} \right)^2 \frac1n s_{yy} \right]       
\end{eqnarray*}
and a similar term for $u(a;y)$.
For $b$ we find
\begin{eqnarray*}
 u(b;x)^2 &=& \sum_{i=1}^n \left(\ddp{b}{x_i}\right)^2 u(x_i)^2 \\
 &=& \sum_{i=1}^n \left( - \ddp{a}{x_i} \bar x - a \frac1n \right)^2 u(x_i)^2 \\
 &=& \left(\bar x\right)^2 u(a;x)^2 + a^2 \frac1n u(x)^2 + 2 u(x)^2 \sum_{i=1}^n \ddp{a}{x_i} \bar x a \frac1n \\
 &=& \left(\bar x\right)^2 u(a;x)^2 + a^2 \frac1n u(x)^2 + 2 u(x)^2 \frac{\bar x a}n \sum_{i=1}^n \left(  \ddp{a}{s_{xx}}  \frac2{n} (x_i - \bar x) + \ddp{a}{s_{xy}} \frac1n (y_i - \bar y)\right) \\
 &=& \left(\bar x\right)^2 u(a;x)^2 + \frac{a^2}n u(x)^2 \\
 u(b;y)^2 &=& \sum_{i=1}^n \left(\ddp{b}{y_i}\right)^2 u(y_i)^2 \\
 &=& \sum_{i=1}^n \left(\frac1n - \ddp{a}{y_i} \bar x\right)^2 u(y_i)^2 \\
 &=& u(y)^2 \frac1n + \left(\bar x \right)^2 u(a;y)^2 - 2 \frac1n u(y)^2 \sum_{i=1}^n \left(  \ddp{a}{s_{yy}}  \frac2{n} (y_i - \bar y) + \ddp{a}{s_{xy}} \frac1n (x_i - \bar x)\right) \\ 
 &=& u(y)^2 \frac1n + \left(\bar x \right)^2 u(a;y)^2
\end{eqnarray*}
For the covariance we have
\begin{eqnarray*}
 \cov(a,b;x) &=& \sum_{i=1}^n \ddp{a}{x_i} \ddp{b}{x_i} u(x_i)^2 \\
  &=&  \sum_{i=1}^n \ddp{a}{x_i}\left( - \ddp{a}{x_i} \bar x - a \frac1n \right) u(x_i)^2 \\
  &=& - u(a;x)^2 \bar x \\
 \cov(a,b;y) &=& \sum_{i=1}^n \ddp{a}{y_i} \ddp{b}{y_i} u(y_i)^2 \\
  &=&  \sum_{i=1}^n \ddp{a}{y_i}\left( \frac1n - \ddp{a}{y_i} \bar x \right) u(y_i)^2 \\
  &=& -u(a;y)^2\bar x
\end{eqnarray*}

\subsection{total least squares - Hessian}
The covariance matrix can be written as the inverse of the Hessian matrix
\begin{equation}
 U_{ij} = \frac12 \ddp{^2W}{\beta_i \beta_j}^{-1}
\end{equation}
where $W$ is the cost function 
\begin{equation*}
 W= \sum_{i=1}^n \frac1{u_y^2} (y_i - a x_i^* - b)^2 + \frac1{u_x^2} (x_i - x_i^*)^2   = \frac1{u_y^2} \underbrace{\sum_{i=1}^n (y_i - a x_i^* - b)^2 + \delta (x_i - x_i^*)^2}_{=S},
\end{equation*} 
and $\beta_i$ are the parameters $a$, $b$ and $x_i^*$.
The second derivatives of the sum of squares $S$ are (using equations \eqref{eq:tls_sum_xstar}, \eqref{eq:tls_sum_xstar^2}, \eqref{eq:tls_xbarybar}
\begin{eqnarray*}
 \frac12 \ddp{^2S}{a^2} &=& \sum_{i=1}^n  (x_i^* )^2 =
 \frac{n}{(\delta+a^2)^2} \left[ a^2 \overline{ y^2}  + 2a \overline{xy} + \overline{x^2} 
-2 a^2b  \bar y  - 2 ab  \bar x + a^2 b^2  \right] \\
&=& \frac{n}{(\delta+a^2)^2} \left[ a^2 \overline{ y^2}  + 2a \overline{xy} + \overline{x^2}
- 2a^2 (\bar y - a \bar x)  \bar y - 2a  \bar x (\bar y- a \bar x ) + a^2  ( \bar y - a \bar x )^2 \right] \\
&=& \frac{n}{(\delta+a^2)^2} \left[ a^2 \overline{ y^2}  +  2a \overline{xy} + \overline{x^2}  \right. 
- 2a^2 (\bar y)^2  +  2a^3 \bar x \bar y
- 2a  \bar x \bar y+  2a^2  (\bar x )^2
\\
&& \left.
+ a^2  ( \bar y - a \bar x )^2 \right] \\
&=& \frac{n}{(\delta+a^2)^2} \left[ a^2 \overline{ y^2}  + 2a \overline{xy} + \overline{x^2}  \right. 
- 2a^2 (\bar y)^2  +  2a^3 \bar x \bar y
- 2a  \bar x \bar y+  2a^2  (\bar x )^2 \\
&& \left. +a^2  (\bar y)^2 - 2a^3 \bar x \bar y + a^4  (\bar x)^2 \right]\\
&=& \frac{n}{(\delta+a^2)^2} \left[ 
a^2 (\overline{ y^2} - (\bar y)^2)  + 2a ( \overline{xy} -  \bar x \bar y) + \overline{x^2} + 2 a^2  (\bar x)^2 + a^4  (\bar x)^2
\right]\\
&=& \frac{n}{(\delta+a^2)^2} \left[ a^2 s_{yy}  + 2a  s_{xy} + s_{xx} + (\bar x)^2 (\delta+a^2)^2\right]
\end{eqnarray*}
\begin{eqnarray*}
 \frac12 \ddp{^2S}{a \partial b} &=& \sum_{i=1}^n  x_i^* = n \bar x  \\
 \frac12 \ddp{^2 S} {b^2} &=& \sum_{i=1}^n 1 = n  \\
  \end{eqnarray*}
\begin{eqnarray*}
 \frac12 \ddp{^2S}{a \partial x_i^*} &=& -(y_i - 2a x_i^* -b) \\
 \frac12 \ddp{^2S}{b \partial x_i^*} &=&  a \\
 \frac12 \ddp{^2S}{x_i^* \partial x_j^*} &=& (\delta+a^2) \delta_{ij}           
 \end{eqnarray*}

\end{document}
